add proofs to test (with admits)

src/Bedrock/Test_X25519_64.v
@@ -6,21 +6,36 @@ Require Import Coq.Lists.List.
 Require Import Crypto.BoundsPipeline.
 Require Import Crypto.Arithmetic.Core.
 Require Import Crypto.Arithmetic.ModOps.
+Require Import Crypto.Bedrock.Tactics.
 Require Import Crypto.Bedrock.Types.
 Require Import Crypto.Bedrock.Translation.Func.
+Require Import Crypto.Bedrock.Util.
+Require Import Crypto.Bedrock.Proofs.Func.
 Require Import Crypto.Language.API.
 Require Import Crypto.Util.ZRange.
 Require Import Crypto.Util.ZUtil.ModInv.
+Require Import Crypto.Util.Tactics.BreakMatch.
 Require Import bedrock2.Syntax.
+Require Import bedrock2.Semantics.
+Require Import coqutil.Word.Interface.
+Require Import coqutil.Word.Properties.
+Require Import coqutil.Map.Interface.
+Require Import coqutil.Map.Properties.
+Require Import bedrock2.Array.
+Require Import bedrock2.Scalars.
 Require Import bedrock2.BasicC64Semantics.
+Require Import bedrock2.ProgramLogic.
+Require Import bedrock2.WeakestPrecondition.
+Require Import bedrock2.WeakestPreconditionProperties.
+Require Import bedrock2.Map.Separation.
 Require bedrock2.NotationsCustomEntry.
-
-Require Import Crypto.Util.Notations.
-Import ListNotations. Local Open Scope Z_scope.
 
 Import Language.Compilers.
 Import Associational Positional.
 Import Types.Notations.
+
+Require Import Crypto.Util.Notations.
+Import ListNotations. Local Open Scope Z_scope.
 
 Local Coercion Z.of_nat : nat >-> Z.
 Local Coercion QArith_base.inject_Z : Z >-> Q.
@@ -92,26 +107,294 @@ Module X25519_64.
     Local Existing Instances Types.rep.Z Types.rep.listZ_mem.
     Let wordsize_bytes := Eval vm_compute in (machine_wordsize / 8)%Z.
 
-    Local Instance p : Types.parameters :=
+    Instance p : Types.parameters :=
       {| semantics := BasicC64Semantics.parameters;
          varname_gen := fun i => String.append "x" (Decimal.decimal_string_of_Z (Z.of_nat i));
          error := expr.var "ERROR";
          word_size_in_bytes := wordsize_bytes;
       |}.
 
-    Definition mulmod_bedrock : cmd :=
-      match mulmod with
-      | ErrorT.Success e =>
-        snd (translate_func e
-                            ("y0", ("y1", tt)) (* argument names *)
-                            (n, (n, tt)) (* lengths for list arguments *)
-                            (expr.var "y0") (* location(s) for returned lists (can be in terms of arguments) *)
-                            "ret") (* return value name *)
-      | ErrorT.Error _ => Syntax.cmd.skip
-      end.
+    Local Definition bedrock_func : Type :=
+      string * (list string * list string * cmd.cmd).
+    Local Coercion name_of_func (f : bedrock_func) := fst f.
+
+    Definition mulmod_bedrock : bedrock_func :=
+      ("mulmod_bedrock",
+       match mulmod with
+       | ErrorT.Success e =>
+         translate_func e
+                        ("in0", ("in1", tt)) (* argument names *)
+                        (n, (n, tt)) (* lengths for list arguments *)
+                        (expr.var "in0") (* location(s) for returned lists (can be in terms of arguments) *)
+                        "ret" (* return value name *)
+       | ErrorT.Error _ => (nil, nil, Syntax.cmd.skip)
+       end).
+
+    Section Proofs.
+
+      (* requires some kind of proof about decimal stringification *)
+      Lemma decimal_varname_gen_unique :
+        forall i j : nat, varname_gen i = varname_gen j <-> i = j.
+      Admitted.
+
+      Instance p_ok : Types.ok.
+      Proof.
+        constructor.
+        { exact BasicC64Semantics.parameters_ok. }
+        { reflexivity. }
+        { exact decimal_varname_gen_unique. }
+      Defined.
+
+      Local Notation M := (s - Associational.eval c)%Z.
+      Local Notation eval :=
+        (eval (weight limbwidth_num limbwidth_den) n).
+      
+      Definition Bignum (addr : Semantics.word) (x : Z) :
+        Semantics.mem -> Prop :=
+        Lift1Prop.ex1
+          (fun xs =>
+             sep (emp (eval (map word.unsigned xs) = x))
+                 (sep (emp (length xs = n))
+                      (array scalar (word.of_Z word_size_in_bytes)
+                             addr xs))).
+
+      (* TODO: Ideally, the translation would take an extra argument for every
+         list in the output, and remove those from the rets. *)
+      (* TODO: it would be nice to say something like (rets = [px]); that
+         returned lists are not just put back in some pointer somewhere that has
+         the right frame, but are put back at exactly the correct pointer *)
+
+      Instance spec_of_mulmod_bedrock : spec_of mulmod_bedrock :=
+        fun functions =>
+          forall x y px py t m
+                 (R : Semantics.mem -> Prop),
+            sep (sep (Bignum px x) (Bignum py y)) R m ->
+            WeakestPrecondition.call
+              (p:=@semantics p)
+              functions mulmod_bedrock t m
+              (px :: py :: nil)
+              (fun t' m' rets =>
+                 t = t' /\
+                 rets = [px]%list /\
+                 sep (sep (Bignum px ((x * y) mod M)%Z)
+                          (Bignum py y)) R m').
+
+      (* TODO: maybe make a computable condition for this *)
+      (* Won't pass right now because valid_expr isn't complete *)
+      Lemma mulmod_valid_func v :
+        mulmod = ErrorT.Success v ->
+        valid_func (v (fun H3 : API.type => unit)).
+      Admitted.
+
+      (* TODO: ask Jason for help *)
+      Lemma mulmod_Wf v :
+        mulmod = ErrorT.Success v ->
+        Wf.Compilers.expr.Wf3 v.
+      Admitted.
+
+      Lemma mulmod_length v (x y : API.interp_type type_listZ) :
+        mulmod = ErrorT.Success v ->
+        length
+          (expr.interp (@Compilers.ident_interp) (v API.interp_type)
+                       x y) = n.
+      Proof.
+        intro Hmm. vm_compute in Hmm.
+        inversion Hmm.
+        vm_compute. reflexivity.
+      Qed.
+
+      (* TODO: here's where we need to use the FC pipeline to say things about
+         correctness *)
+      (* this can be changed to use type.app_curried if that's easier *)
+      Lemma mulmod_correct v x y :
+        mulmod = ErrorT.Success v ->
+        eval
+          (map word.wrap
+               (expr.interp
+                  (@Compilers.ident_interp) (v API.interp_type)
+                  (map word.unsigned x) (map word.unsigned y))) =
+        ((eval (map word.unsigned x) * eval (map word.unsigned y)) mod M)%Z.
+      Admitted.
+
+      (* TODO : move *)
+      Lemma substring_0_0 :
+        forall s, substring 0 0 s = "".
+      Proof.
+        clear. destruct s; reflexivity.
+      Qed.
+
+      Lemma varname_gen_startswith v i :
+        v = varname_gen i ->
+        String.startswith "x" v = true.
+      Proof.
+        cbn [varname_gen p]. intro.
+        subst. cbn. rewrite substring_0_0.
+        reflexivity.
+      Qed.
+
+      (* TODO : move *)
+      Lemma map_of_Z_unsigned x :
+        map word.of_Z (map word.unsigned x) = x.
+      Proof.
+        rewrite map_map.
+        rewrite map_ext with (g:=id);
+          [ solve [apply map_id] | ].
+        intros. rewrite word.of_Z_unsigned.
+        reflexivity.
+      Qed.
+
+      (* TODO : move *)
+      Lemma map_unsigned_of_Z x :
+        map word.unsigned (map word.of_Z x) = map word.wrap x.
+      Proof.
+        rewrite map_map. apply map_ext.
+        exact word.unsigned_of_Z.
+      Qed.
+
+      Lemma mulmod_bedrock_correct :
+        program_logic_goal_for_function! mulmod_bedrock.
+      Proof.
+        cbv [program_logic_goal_for spec_of_mulmod_bedrock].
+        cbn [name_of_func mulmod_bedrock fst]. intros.
+        cbv [mulmod_bedrock].
+        case_eq mulmod;
+          [ | let H := fresh in
+              intros ? H; vm_compute in H; congruence ].
+        intros. cbv [Bignum] in * |-. sepsimpl.
+        eapply Proper_call.
+        2:{
+          let xs := match goal with
+                      Hx : eval ?xs = x |- _ =>
+                      xs end in
+          let ys := match goal with
+                      Hy : eval ?ys = y |- _ =>
+                      ys end in
+          apply translate_func_correct
+            with (args:=(xs, (ys, tt)))
+                 (Ra:=R) (Rr:=sep (Bignum py y) R).
+          { apply mulmod_valid_func; eauto. }
+          { apply mulmod_Wf; eauto. }
+          { cbn [LoadStoreList.list_lengths_from_args
+                   LoadStoreList.list_lengths_from_value
+                   fst snd].
+            rewrite !map_length.
+            repeat match goal with H : length _ = n |- _ =>
+                                   rewrite H end.
+            reflexivity. }
+          { intros.
+            cbn [fst snd Types.varname_set_args Types.varname_set
+                     Types.rep.varname_set Types.rep.listZ_mem
+                     Types.rep.Z].
+            cbv [PropSet.union PropSet.singleton_set PropSet.elem_of
+                               PropSet.empty_set].
+            destruct 1 as [? | [? | ?] ]; try tauto;
+              match goal with H : _ = varname_gen _ |- _ =>
+                              apply varname_gen_startswith in H;
+                                vm_compute in H; congruence
+              end. }
+          { cbn [fst snd Types.equivalent_flat_args Types.rep.listZ_mem
+                     Types.equivalent_flat_base Types.rep.equiv
+                     Types.rep.Z]. sepsimpl.
+            exists 1%nat. cbn [firstn skipn length hd].
+            apply SeparationLogic.sep_comm.
+            apply SeparationLogic.sep_assoc.
+            apply SeparationLogic.sep_comm.
+            apply SeparationLogic.sep_ex1_l.
+            exists 1%nat. cbn [firstn skipn length hd].
+            apply SeparationLogic.sep_assoc.
+            sepsimpl; try reflexivity; [ ].
+            eexists. sepsimpl; try reflexivity; [ ].
+            apply SeparationLogic.sep_comm.
+            apply SeparationLogic.sep_assoc.
+            apply SeparationLogic.sep_comm.
+            sepsimpl; try reflexivity; [ ].
+            eexists. sepsimpl; try reflexivity; [ ].
+            rewrite !map_of_Z_unsigned.
+            rewrite !word.of_Z_unsigned in *.
+            change parameters with semantics in *.
+            SeparationLogic.ecancel_assumption. }
+          { cbn. repeat constructor; cbn [In]; try tauto.
+            destruct 1; congruence. }
+          { intros.
+            cbn [fst snd Types.varname_set type.final_codomain
+                     Types.rep.varname_set Types.rep.listZ_mem
+                     Types.rep.Z].
+            cbv [PropSet.singleton_set PropSet.elem_of PropSet.empty_set].
+            intro;
+              match goal with H : _ = varname_gen _ |- _ =>
+                              apply varname_gen_startswith in H;
+                                vm_compute in H; congruence
+              end. }
+          { cbn. repeat constructor; cbn [In]; tauto. }
+          { cbn. rewrite union_empty_r.
+            apply disjoint_singleton_r_iff.
+            cbv [PropSet.singleton_set PropSet.elem_of PropSet.union].
+            destruct 1; congruence. }
+          { cbn - [semantics Semantics.word p].
+            cbv [Bignum].
+            sepsimpl.
+            (let xs := (match goal with
+                          Hx : eval ?xs = x |- _ =>
+                          xs end) in
+             exists xs).
+            sepsimpl;
+              [ rewrite map_length, mulmod_length by assumption;
+                congruence | ].
+            exists (word.unsigned px). sepsimpl.
+            { apply get_put_diff; [ congruence | ].
+              apply get_put_same, word.of_Z_unsigned. }
+
+            eexists. sepsimpl; eauto; [ ].
+            rewrite map_of_Z_unsigned, word.of_Z_unsigned.
+            change parameters with semantics in *.
+            SeparationLogic.ecancel_assumption. } }
+        repeat intro; cbv beta in *.
+        cbn [Types.equivalent_flat_base
+               Types.rep.equiv Types.rep.listZ_mem Types.rep.Z
+               type.final_codomain] in *.
+        repeat match goal with
+               | _ => progress subst
+               | _ => progress sepsimpl_hyps
+               | H : _ /\ _ |- _ => destruct H
+               | |- _ /\ _ => split; [ reflexivity | ]
+               end.
+        (* see TODO above spec *)
+        match goal with
+          |- ?rets = [px]%list /\ _ =>
+          assert (rets = [px]%list) by admit;
+            split; [ assumption | subst ]
+        end.
+        sepsimpl.
+        match goal with
+        | H : dexpr _ _ (expr.literal _) _ |- _ =>
+          cbn [dexpr WeakestPrecondition.expr expr_body hd] in H;
+            cbv [literal] in H; rewrite word.of_Z_unsigned in H;
+              inversion H; clear H; subst
+        end.
+        match goal with
+        | H : sep ?p (sep ?q ?r) ?m
+          |- sep (sep _ ?q) ?r ?m =>
+          eapply SeparationLogic.sep_assoc;
+            eapply SeparationLogic.Proper_sep_impl1;
+            [ | reflexivity | eapply H ]; [ ];
+            clear H; repeat intro
+        end.
+        cbv [Bignum].
+        eexists; sepsimpl;
+          [ | | eassumption];
+          [ | cbn [type.app_curried];
+              rewrite map_length, mulmod_length; solve [eauto] ].
+        clear H.
+        cbn [type.app_curried fst snd].
+        rewrite map_unsigned_of_Z.
+        apply mulmod_correct; eauto.
+      Admitted.
+
+    End Proofs.
 
     Import NotationsCustomEntry.
     Local Set Printing Width 150.
     Redirect "Crypto.Bedrock.Test_X25519_64.mulmod_bedrock" Compute mulmod_bedrock.
+
   End __.
 End X25519_64.
